our_cook/encoding.v
@@ -12,51 +12,55 @@ Fixpoint incRefs (n : nat) (m : nat) (refs : list (nat * nat)) :=
 
 Fixpoint findRef (n : nat) (refs : list (nat * nat)) :=
   match refs with
-  | [] => n 
-  | (x, y) :: ps => 
+  | [] => 42 (* this case should never happen *)
+  | (x, y) :: ps =>
       if n =? x 
       then y
       else findRef n ps
   end.
   
 Definition pointer (p : proc) :=
-  Rep (In 0 (In 0 (In 1 p))).
+  Rep (In (BN 0) (In (BN 0) (In (BN 1) p))).
 
 Fixpoint encode (s : term) (u r : nat) (refs : list (nat * nat)) :=
   match s with
-  | Abs s => Out u (In 0 (In 1 (In 2 (encode s 2 1 ((0,0) :: incRefs 1 4 refs)))))
+  | Abs s => Out (BN u) (In (BN 0) (In (BN 1) (In (BN 2) (encode s 2 1 ((0,0) :: incRefs 1 4 refs)))))
   | App s v => (Res ^^ 4) (Par 
-      (In 3 (In 2 (Out 1 (Out 2 (Out 3 (Par
-        (Link 2 (9 + u))
+      (In (BN 3) (In (BN 2) (Out (BN 1) (Out (BN 2) (Out (BN 3) (Par
+        (Link (BN 2) (BN (9 + u)))
         (Par
-          (Link 1 (9 + r))
-          (Link 0 3)
+          (Link (BN 1) (BN (9 + r)))
+          (Link (BN 0) (BN 3))
         )
       ))))))
       (Par
         (encode s 3 2 (incRefs 0 4 refs))
-        (Out 1 (encode_value v (incRefs 0 4 refs)))
+        (Out (BN 1) (encode_value v (incRefs 0 4 refs)))
       )
     )
   | Force v => (Res ^^ 2) (Par
-      (Out 1 (encode_value v (incRefs 0 2 refs)))
-      (In 1 (Out 0 (Out 0 (Out 1 (Par
-        (Link 1 (6 + u))
-        (Link 0 (6 + r))
+      (Out (BN 1) (encode_value v (incRefs 0 2 refs)))
+      (In (BN 1) (Out (BN 0) (Out (BN 0) (Out (BN 1) (Par
+        (Link (BN 1) (BN (6 + u)))
+        (Link (BN 0) (BN (6 + r)))
       )))))
     )
-  | Ret v => Out r (encode_value v refs)
+  | Ret v => Out (BN r) (encode_value v refs)
   | Bind s t => (Res ^^ 2) (Par
       (encode s 1 0 (incRefs 0 2 refs))
-      (In 0 (encode t (3 + u) (3 + r) ((0,0) :: incRefs 1 3 refs)))
+      (In (BN 0) (encode t (3 + u) (3 + r) ((0,0) :: incRefs 1 3 refs)))
     )
-  | Val v => Out u (encode_value v refs)
+  | Val v => Out (BN u) (encode_value v refs)
   end
 
 with encode_value (v : value) (refs : list (nat * nat)) :=
   pointer(
     match v with
-    | Var n => Link 0 (findRef n refs + 4)
+    | Var n => 
+      match n with
+      | (BV m) => Link (BN 0) (BN (findRef m refs + 4))
+      | (FV m) => Link (BN 0) (FN m)
+      end
     | Thunk s => encode s 1 0 (incRefs 0 4 refs)
     end
   ).
@@ -64,3 +68,5 @@ with encode_value (v : value) (refs : list (nat * nat)) :=
 Notation "$ v ; refs $" := (encode_value v refs) (at level 90, left associativity).
 
 Notation "$ s ; u ; r ; refs $" := (encode s u r refs) (at level 90, left associativity).
+
+Definition encode' (s : term) := Res (Res ($ s ; 1 ; 0 ; [] $)).
